Extend the notion of sorts to handle HTS/2TT

theories/Sorts.v
@@ -7,7 +7,9 @@ From Translation Require Import util.
 Class notion := {
   sort : Type ;
   succ : sort -> sort ;
-  max : sort -> sort -> sort ;
+  prod_sort : sort -> sort -> sort ;
+  sum_sort : sort -> sort -> sort ;
+  eq_sort : sort -> sort ;
   eq_dec : forall s z : sort, {s = z} + {s <> z} ;
   succ_inj : forall s z, succ s = succ z -> s = z
 }.
@@ -15,7 +17,9 @@ Class notion := {
 Local Instance nat_sorts : notion := {|
   sort := nat ;
   succ := S ;
-  max := Nat.max ;
+  prod_sort := Nat.max ;
+  sum_sort := Nat.max ;
+  eq_sort s := s ;
   eq_dec := Nat.eq_dec
 |}.
 Proof.
@@ -25,9 +29,75 @@ Defined.
 Local Instance type_in_type : notion := {|
   sort := unit ;
   succ u := u ;
-  max u v := tt
+  prod_sort u v := tt ;
+  sum_sort u v := tt ;
+  eq_sort s := tt
 |}.
 Proof.
   - intros [] []. left. reflexivity.
   - intros [] [] _. reflexivity.
 Defined.
+
+Inductive univ := sType (n : nat) | sProp.
+Local Instance fixed_sorts : notion := {|
+  sort := univ ;
+  succ s := 
+    match s with 
+    | sType n => sType (S n)
+    | sProp => sProp
+    end ;
+  prod_sort s1 s2 :=
+    match s1, s2 with
+    | sType n, sType m => sType (Nat.max n m)
+    | _, sProp => sProp
+    | sProp, sType n => sType n
+    end ;
+  sum_sort s1 s2 :=
+    match s1, s2 with
+    | sType n, sType m => sType (Nat.max n m)
+    | sType n, sProp => sType n
+    | sProp, sType n => sType n
+    | sProp, sProp => sProp
+    end ;
+  eq_sort s := s
+|}.
+Proof.
+  - intros s z. decide equality. decide equality.
+  - intros s z e.
+    destruct s, z ; inversion e ; eauto.
+Defined.
+
+Inductive twolevel := F (n : nat) | U (n : nat).
+Local Instance twolevel_sorts : notion := {|
+  sort := twolevel ;
+  succ s := 
+    match s with 
+    | U n => U (S n)
+    | F n => F (S n)
+    end ;
+  prod_sort s1 s2 :=
+    match s1, s2 with
+    | U n, U m => U (Nat.max n m)
+    | F n, F m => F (Nat.max n m)
+    | U n, F m => U (Nat.max n m)
+    | F n, U m => U (Nat.max n m)
+    end ;
+  sum_sort s1 s2 :=
+    match s1, s2 with
+    | U n, U m => U (Nat.max n m)
+    | F n, F m => F (Nat.max n m)
+    | U n, F m => U (Nat.max n m)
+    | F n, U m => U (Nat.max n m)
+    end ;
+  eq_sort s :=
+    match s with
+    | U n => U n
+    | F n => U n
+    end
+|}.
+Proof.
+  - intros s z. decide equality ; decide equality.
+  - intros s z e.
+    destruct s, z ; inversion e ; eauto.
+Defined.
+
